Write Integration Tests & Refactor Get Keys

AwsCryptographicMaterialProviders/dafny/AwsCryptographyKeyStore/test/TestCreateKeys.dfy
@@ -4,6 +4,7 @@
 include "../src/Index.dfy"
 include "Fixtures.dfy"
 include "CleanupItems.dfy"
+include "TestGetKeys.dfy"
 
 module {:options "/functionSyntax:4" } TestCreateKeys {
   import Types = AwsCryptographyKeyStoreTypes
@@ -20,6 +21,7 @@ module {:options "/functionSyntax:4" } TestCreateKeys {
   import KmsArn
   import UUID
   import AwsArnParsing
+  import TestGetKeys
 
   /*
     // If you need to re-create the MRK Branch Keys
@@ -93,101 +95,14 @@ module {:options "/functionSyntax:4" } TestCreateKeys {
                                                    branchKeyIdentifier := None,
                                                    encryptionContext := None
                                                  ));
-    var beaconKeyResult :- expect keyStore.GetBeaconKey(
-      Types.GetBeaconKeyInput(
-        branchKeyIdentifier := branchKeyId.branchKeyIdentifier
-      ));
 
-    var activeResult :- expect keyStore.GetActiveBranchKey(
-      Types.GetActiveBranchKeyInput(
-        branchKeyIdentifier := branchKeyId.branchKeyIdentifier
-      ));
-
-    var branchKeyVersion :- expect UTF8.Decode(activeResult.branchKeyMaterials.branchKeyVersion);
-    var versionResult :- expect keyStore.GetBranchKeyVersion(
-      Types.GetBranchKeyVersionInput(
-        branchKeyIdentifier := branchKeyId.branchKeyIdentifier,
-        branchKeyVersion := branchKeyVersion
-      ));
-
-    var encryptedActive :- expect keyStore.config.storage.GetEncryptedActiveBranchKey(
-      Types.GetEncryptedActiveBranchKeyInput(
-        Identifier := branchKeyId.branchKeyIdentifier
-      )
+    // Get branch key items from storage
+    TestGetKeys.VerifyGetKeys(
+      identifier := branchKeyId.branchKeyIdentifier,
+      keyStore := keyStore,
+      storage := keyStore.config.storage,
+      ddbClient := ddbClient
     );
-
-    var encryptedVersion :- expect keyStore.config.storage.GetEncryptedBranchKeyVersion(
-      Types.GetEncryptedBranchKeyVersionInput(
-        Identifier := branchKeyId.branchKeyIdentifier,
-        Version := encryptedActive.Item.Type.ActiveHierarchicalSymmetricVersion.Version
-      )
-    );
-
-    var encryptedBeacon :- expect keyStore.config.storage.GetEncryptedBeaconKey(
-      Types.GetEncryptedBeaconKeyInput(
-        Identifier := branchKeyId.branchKeyIdentifier
-      )
-    );
-
-    //= aws-encryption-sdk-specification/framework/branch-key-store.md#branch-key-and-beacon-key-creation
-    //= type=test
-    //# This timestamp MUST be in ISO 8601 format in UTC, to microsecond precision (e.g. “YYYY-MM-DDTHH:mm:ss.ssssssZ“)
-    expect ISO8601?(encryptedActive.Item.CreateTime);
-    expect ISO8601?(encryptedVersion.Item.CreateTime);
-    expect ISO8601?(encryptedBeacon.Item.CreateTime);
-
-    // Since this process uses a read DDB table,
-    // the number of records will forever increase.
-    // To avoid this, remove the items.
-    var _ := CleanupItems.DeleteBranchKey(Identifier:=branchKeyId.branchKeyIdentifier, ddbClient:=ddbClient);
-
-    expect beaconKeyResult.beaconKeyMaterials.beaconKey.Some?;
-    expect |beaconKeyResult.beaconKeyMaterials.beaconKey.value| == 32;
-    expect |activeResult.branchKeyMaterials.branchKey| == 32;
-    expect versionResult.branchKeyMaterials.branchKey == activeResult.branchKeyMaterials.branchKey;
-    expect versionResult.branchKeyMaterials.branchKeyIdentifier
-        == activeResult.branchKeyMaterials.branchKeyIdentifier
-        == beaconKeyResult.beaconKeyMaterials.beaconKeyIdentifier;
-    expect versionResult.branchKeyMaterials.branchKeyVersion == activeResult.branchKeyMaterials.branchKeyVersion;
-
-    //= aws-encryption-sdk-specification/framework/branch-key-store.md#createkey
-    //= type=test
-    //# If no branch key id is provided,
-    //# then this operation MUST create a [version 4 UUID](https://www.ietf.org/rfc/rfc4122.txt)
-    //# to be used as the branch key id.
-    var idByteUUID :- expect UUID.ToByteArray(activeResult.branchKeyMaterials.branchKeyIdentifier);
-    var idRoundTrip :- expect UUID.FromByteArray(idByteUUID);
-    expect idRoundTrip == activeResult.branchKeyMaterials.branchKeyIdentifier;
-
-
-    //= aws-encryption-sdk-specification/framework/branch-key-store.md#branch-key-and-beacon-key-creation
-    //= type=test
-    //# This guid MUST be [version 4 UUID](https://www.ietf.org/rfc/rfc4122.txt)
-    var versionString :- expect UTF8.Decode(activeResult.branchKeyMaterials.branchKeyVersion);
-    var versionByteUUID :- expect UUID.ToByteArray(versionString);
-    var versionRoundTrip :- expect UUID.FromByteArray(versionByteUUID);
-    expect versionRoundTrip == versionString;
-
-  }
-
-  lemma ISO8601Test()
-  {
-    assert ISO8601?("2024-08-06T17:23:25.000874Z");
-  }
-
-  predicate ISO8601?(
-    CreateTime: string
-  )
-  {
-    // “YYYY-MM-DDTHH:mm:ss.ssssssZ“
-    && |CreateTime| == 27
-    && CreateTime[4] == '-'
-    && CreateTime[7] == '-'
-    && CreateTime[10] == 'T'
-    && CreateTime[13] == ':'
-    && CreateTime[16] == ':'
-    && CreateTime[19] == '.'
-    && CreateTime[26] == 'Z'
   }
 
   method {:test} TestCreateOptions()
