AwsCryptographicMaterialProviders/dafny/AwsCryptographyKeyStore/test/TestGetKeys.dfy
@@ -3,6 +3,7 @@
 
 include "../src/Index.dfy"
 include "Fixtures.dfy"
+include "CleanupItems.dfy"
 include "../src/ErrorMessages.dfy"
 
 // TODO-HV2-M1: add more HV2 tests.
@@ -18,8 +19,93 @@ module TestGetKeys {
   import opened Fixtures
   import UTF8
   import ErrorMessages = KeyStoreErrorMessages
+  import UUID
+  import CleanupItems
 
   const incorrectLogicalName := "MySuperAwesomeTableName"
+
+  method VerifyGetKeys(
+    identifier : string,
+    keyStore : Types.IKeyStoreClient,
+    storage : Types.IKeyStorageInterface,
+    ddbClient : DDB.Types.IDynamoDBClient
+  ) {
+   var beaconKeyResult :- expect keyStore.GetBeaconKey(
+      Types.GetBeaconKeyInput(
+        branchKeyIdentifier := identifier
+      ));
+
+    var activeResult :- expect keyStore.GetActiveBranchKey(
+      Types.GetActiveBranchKeyInput(
+        branchKeyIdentifier := identifier
+      ));
+
+    var branchKeyVersion :- expect UTF8.Decode(activeResult.branchKeyMaterials.branchKeyVersion);
+    var versionResult :- expect keyStore.GetBranchKeyVersion(
+      Types.GetBranchKeyVersionInput(
+        branchKeyIdentifier := identifier,
+        branchKeyVersion := branchKeyVersion
+      ));
+
+    var encryptedActive :- expect storage.GetEncryptedActiveBranchKey(
+      Types.GetEncryptedActiveBranchKeyInput(
+        Identifier := identifier
+      )
+    );
+
+    expect encryptedActive.Item.Type.ActiveHierarchicalSymmetricVersion?;
+    var encryptedVersion :- expect storage.GetEncryptedBranchKeyVersion(
+      Types.GetEncryptedBranchKeyVersionInput(
+        Identifier := identifier,
+        Version := encryptedActive.Item.Type.ActiveHierarchicalSymmetricVersion.Version
+      )
+    );
+
+    var encryptedBeacon :- expect storage.GetEncryptedBeaconKey(
+      Types.GetEncryptedBeaconKeyInput(
+        Identifier := identifier
+      )
+    );
+
+    //= aws-encryption-sdk-specification/framework/branch-key-store.md#branch-key-and-beacon-key-creation
+    //= type=test
+    //# This timestamp MUST be in ISO 8601 format in UTC, to microsecond precision (e.g. “YYYY-MM-DDTHH:mm:ss.ssssssZ“)
+    expect ISO8601?(encryptedActive.Item.CreateTime);
+    expect ISO8601?(encryptedVersion.Item.CreateTime);
+    expect ISO8601?(encryptedBeacon.Item.CreateTime);
+
+    // Since this process uses a read DDB table,
+    // the number of records will forever increase.
+    // To avoid this, remove the items.
+    var _ := CleanupItems.DeleteBranchKey(Identifier:=identifier, ddbClient:=ddbClient);
+
+    expect beaconKeyResult.beaconKeyMaterials.beaconKey.Some?;
+    expect |beaconKeyResult.beaconKeyMaterials.beaconKey.value| == 32;
+    expect |activeResult.branchKeyMaterials.branchKey| == 32;
+    expect versionResult.branchKeyMaterials.branchKey == activeResult.branchKeyMaterials.branchKey;
+    expect versionResult.branchKeyMaterials.branchKeyIdentifier
+        == activeResult.branchKeyMaterials.branchKeyIdentifier
+        == beaconKeyResult.beaconKeyMaterials.beaconKeyIdentifier;
+    expect versionResult.branchKeyMaterials.branchKeyVersion == activeResult.branchKeyMaterials.branchKeyVersion;
+
+    //= aws-encryption-sdk-specification/framework/branch-key-store.md#createkey
+    //= type=test
+    //# If no branch key id is provided,
+    //# then this operation MUST create a [version 4 UUID](https://www.ietf.org/rfc/rfc4122.txt)
+    //# to be used as the branch key id.
+    var idByteUUID :- expect UUID.ToByteArray(activeResult.branchKeyMaterials.branchKeyIdentifier);
+    var idRoundTrip :- expect UUID.FromByteArray(idByteUUID);
+    expect idRoundTrip == activeResult.branchKeyMaterials.branchKeyIdentifier;
+
+
+    //= aws-encryption-sdk-specification/framework/branch-key-store.md#branch-key-and-beacon-key-creation
+    //= type=test
+    //# This guid MUST be [version 4 UUID](https://www.ietf.org/rfc/rfc4122.txt)
+    var versionString :- expect UTF8.Decode(activeResult.branchKeyMaterials.branchKeyVersion);
+    var versionByteUUID :- expect UUID.ToByteArray(versionString);
+    var versionRoundTrip :- expect UUID.FromByteArray(versionByteUUID);
+    expect versionRoundTrip == versionString;
+  }
 
   method {:test} TestGetBeaconKey()
   {
@@ -383,5 +469,25 @@ module TestGetKeys {
       ));
 
     expect |activeResult.branchKeyMaterials.branchKey| == 32;
+  }
+
+  lemma ISO8601Test()
+  {
+    assert ISO8601?("2024-08-06T17:23:25.000874Z");
+  }
+
+  predicate method ISO8601?(
+    CreateTime: string
+  )
+  {
+    // “YYYY-MM-DDTHH:mm:ss.ssssssZ“
+    && |CreateTime| == 27
+    && CreateTime[4] == '-'
+    && CreateTime[7] == '-'
+    && CreateTime[10] == 'T'
+    && CreateTime[13] == ':'
+    && CreateTime[16] == ':'
+    && CreateTime[19] == '.'
+    && CreateTime[26] == 'Z'
   }
 }
